veric/semax_ext.v
@@ -21,17 +21,18 @@ Variable Z : Type.
 
 Variable Espec : juicy_ext_spec Z.
 
-Variable gx : genv.
-
 Definition funspec2types id (A : Type) (ef : external_function) : Type :=
   if ident_eq id (ef_id ef) then A else (ext_spec_type Espec ef).
 
-Definition funspec2pre (A : Type) P id ef x (tys : list typ) args (z : Z) m : Prop :=
+Parameter symb2genv : forall (ge_s : PTree.t block), genv. (*TODO*)
+Axiom symb2genv_ax : forall (ge_s : PTree.t block), Genv.genv_symb (symb2genv ge_s) = ge_s.
+
+Definition funspec2pre (A : Type) P id ef x ge_s (tys : list typ) args (z : Z) m : Prop :=
   match ident_eq id (ef_id ef) as s 
   return ((if s then A else ext_spec_type Espec ef) -> Prop)
   with 
-    | left _ => fun x' => P x' (make_ext_args gx 1 args) (m_phi m)
-    | right n => fun x' => ext_spec_pre Espec ef x' tys args z m
+    | left _ => fun x' => P x' (make_ext_args (symb2genv ge_s) 1 args) (m_phi m)
+    | right n => fun x' => ext_spec_pre Espec ef x' ge_s tys args z m
   end x.
 
 Definition funspec2post (A : Type) Q id ef x (tret : option typ) ret (z : Z) m : Prop :=
@@ -56,14 +57,17 @@ Definition funspec2extspec (f : (ident*funspec))
 Definition wf_funspec (f : funspec) :=
   match f with
     | mk_funspec sig A P Q => 
-      forall a rho rho' phi phi', 
-        P a rho phi -> Q a rho' phi' -> 
+        (forall a rho rho' phi phi', 
+        (P a rho phi -> Q a rho' phi' -> 
         forall adr, 
           match phi @ adr with
             | NO _ => True
             | YES _ _ _ _ => True
             | PURE k pp => phi' @ adr = PURE k (preds_fmap (approx (level phi')) pp)
-          end
+          end))
+        /\ (forall a ge ge' n args phi, Genv.genv_symb ge = Genv.genv_symb ge' ->
+              (P a (make_ext_args ge n args) phi <-> 
+               P a (make_ext_args ge' n args) phi))
   end.
 
 Program Definition funspec2jspec f (wf : wf_funspec (snd f)) : juicy_ext_spec Z :=
@@ -95,7 +99,8 @@ revert wf; unfold wf_funspec; simpl; intros H2. revert t H H0 H2.
 unfold funspec2pre, funspec2post. 
 destruct (ident_eq i (ef_id e)).
 * intros. intros adr.
-specialize (H2 t (make_ext_args gx 1 args) (make_ext_rval 1 rv)). 
+destruct H2 as [H2 _].
+specialize (H2 t (make_ext_args (symb2genv ge_s) 1 args) (make_ext_rval 1 rv)). 
 apply (H2 (m_phi jm) (m_phi jm') H H0 adr).
 * destruct Espec; simpl; intros.
 clear H2; eapply (JE_rel e); eauto.
@@ -145,21 +150,22 @@ Fixpoint funspecs_norepeat fs :=
 Lemma in_funspecs_wf f fs : in_funspecs f fs -> wf_funspec (snd f).
 Proof. induction fs; simpl; inversion 1; try subst f0; auto. Qed.
 
-Fixpoint add_funspecs_rec (Z : Type) (Espec : juicy_ext_spec Z) gx (fs : wf_funspecs) :=
+Fixpoint add_funspecs_rec (Z : Type) (Espec : juicy_ext_spec Z) (fs : wf_funspecs) :=
   match fs with
     | wf_nil => Espec
-    | wf_cons (i,f) wf fs' => funspec2jspec Z (add_funspecs_rec Z Espec gx fs') gx (i,f) wf
+    | wf_cons (i,f) wf fs' => 
+      funspec2jspec Z (add_funspecs_rec Z Espec fs') (i,f) wf
   end.
 
 Require Import JMeq.
 
-Lemma add_funspecs_pre {Z gx fs id sig A P Q x args m} Espec tys :
+Lemma add_funspecs_pre {Z fs id sig A P Q x args m} Espec tys ge_s :
   let ef := EF_external id (funsig2signature sig) in
   funspecs_norepeat fs -> 
   in_funspecs (id, (mk_funspec sig A P Q)) fs -> 
-  P x (make_ext_args gx 1%positive args) (m_phi m) ->
-  exists x' : ext_spec_type (JE_spec _ (add_funspecs_rec Z Espec gx fs)) ef, 
-    JMeq x x' /\ forall z, ext_spec_pre (add_funspecs_rec Z Espec gx fs) ef x' tys args z m.
+  P x (make_ext_args (symb2genv ge_s) 1%positive args) (m_phi m) ->
+  exists x' : ext_spec_type (JE_spec _ (add_funspecs_rec Z Espec fs)) ef, 
+    JMeq x x' /\ forall z, ext_spec_pre (add_funspecs_rec Z Espec fs) ef x' ge_s tys args z m.
 Proof.
 induction fs; [intros; elimtype False; auto|]; intros ef H H1 H2.
 destruct H1 as [H1|H1].
@@ -188,11 +194,11 @@ destruct (ident_eq i id).
 }
 Qed.
 
-Lemma add_funspecs_post {Z Espec tret gx fs id sig A P Q x ret m z} :
+Lemma add_funspecs_post {Z Espec tret fs id sig A P Q x ret m z} :
   let ef := EF_external id (funsig2signature sig) in
   funspecs_norepeat fs -> 
   in_funspecs (id, (mk_funspec sig A P Q)) fs -> 
-  ext_spec_post (add_funspecs_rec Z Espec gx fs) ef x tret ret z m -> 
+  ext_spec_post (add_funspecs_rec Z Espec fs) ef x tret ret z m -> 
   exists x' : A, 
     JMeq x x' /\ Q x' (make_ext_rval 1%positive ret) (m_phi m).
 Proof.
@@ -222,10 +228,10 @@ destruct (ident_eq i id).
 }
 Qed.
 
-Definition add_funspecs (Espec : OracleKind) gx (fs : wf_funspecs) : OracleKind :=
+Definition add_funspecs (Espec : OracleKind) (fs : wf_funspecs) : OracleKind :=
   match Espec with
     | Build_OracleKind ty spec => 
-      Build_OracleKind ty (add_funspecs_rec ty spec gx fs)
+      Build_OracleKind ty (add_funspecs_rec ty spec fs)
   end.
 
 Definition local_funspec (f : funspec) :=
@@ -246,15 +252,12 @@ Section semax_ext.
 
 Variable Espec : OracleKind.
 
-(*[NOTE genv]: semax_external should be parameterized by gx. *)
-
-Lemma semax_ext gx id sig A P Q (fs : wf_funspecs) : 
+Lemma semax_ext id sig A P Q (fs : wf_funspecs) : 
   let f := mk_funspec sig A P Q in
   local_funspec f -> 
   in_funspecs (id,f) fs -> 
   funspecs_norepeat fs -> 
-  (forall n, semax_external (add_funspecs Espec gx fs) 
-                            (EF_external id (funsig2signature sig)) _ P Q n).
+  (forall n, semax_external (add_funspecs Espec fs) (EF_external id (funsig2signature sig)) _ P Q n).
 Proof.
 intros f Hloc Hin Hnorepeat.
 unfold semax_external.
@@ -262,9 +265,13 @@ intros n ge x n0 Hlater F ts args jm H jm' H2 H3.
 destruct H3 as [s [t [Hjoin [Hp Hf]]]].
 cut (P x (make_ext_args ge 1 args) (m_phi jm')). intro Hp'.
 destruct Espec.
-destruct (add_funspecs_pre OK_spec ts Hnorepeat Hin Hp') as [x' [Heq Hpre]].
+assert (Hp'': P x (make_ext_args (symb2genv (Genv.genv_symb ge)) 1 args) (m_phi jm')).
+{ generalize (in_funspecs_wf _ _ Hin). simpl; intros [Hwf1 Hwf2].
+  rewrite Hwf2; eauto.
+  rewrite symb2genv_ax; auto. }
+destruct (add_funspecs_pre OK_spec ts (Genv.genv_symb ge) Hnorepeat Hin Hp'') 
+  as [x' [Heq Hpre]].
 simpl.
-assert (ge = gx) as <- by admit. (*cf. [NOTE genv]*)
 exists x'.
 intros z.
 split; [solve[apply Hpre]|].
@@ -284,7 +291,7 @@ split; auto. destruct F. simpl in Hf|-*. eapply h in Hf; eauto.
 eapply add_funspecs_post in Hpost; eauto.
 destruct Hpost as [x'' [Heq' Hq']].
 assert (JMeq x x'') by (eapply JMeq_trans; eauto).
-solve[apply JMeq_eq in H1; subst; auto].
+solve[apply JMeq_eq in H0; subst; auto].
 
 unfold f in Hloc; destruct Hloc as [Hloc _]. 
 solve[eapply Hloc; eauto].
