veric/SequentialClight.v
@@ -21,7 +21,7 @@ Definition dryspec : ext_spec unit :=
      (*ext_spec_type*)
      (fun ef => False)
      (*ext_spec_pre*)
-     (fun ef Hef tys vl m z => False) 
+     (fun ef Hef ge tys vl m z => False) 
      (*ext_spec_post*)
      (fun ef Hef ty vl m z => False)
      (*ext_spec_exit*)
